regcol_lookup

theories/automation.v
@@ -486,7 +486,29 @@ Global Hint Extern 10 (TacticHint (regcol_compute_hint _ _)) =>
   subst_remembered;
   apply H : typeclass_instances.
 
-(** * [regcol cancellation] *)
+(** * functions to compute on a regcol *)
+Fixpoint regcol_lookup (r : reg_kind) (regs : list (reg_kind * valu_shape)) : option (valu_shape) :=
+  match regs with
+  | (r', s)::regs' =>
+      if reg_kind_eqb r r' then
+        Some s
+      else
+        regcol_lookup r regs'
+  | [] => None
+  end.
+Lemma regcol_lookup_Some `{!islaG Σ} `{!threadG} r regs s:
+  regcol_lookup r regs = Some s →
+  reg_col regs -∗ ∃ v, ⌜valu_has_shape v s⌝ ∗ r ↦ᵣₖ v ∗ (r ↦ᵣₖ v -∗ reg_col regs).
+Proof.
+  iIntros (Hr) "Hregs". iInduction regs as [|[r' s'] regs'] "IH" forall (s Hr) => //.
+  rewrite ->reg_col_cons. iDestruct "Hregs" as "[[%v [% Hv]] Hregs]".
+  simpl in *. rewrite reg_kind_eqb_eq in Hr. case_bool_decide; simplify_eq/=.
+  { iExists _. rewrite ->reg_col_cons => /=. iFrame. eauto with iFrame. }
+  iDestruct ("IH" with "[//] Hregs") as (v' ?) "[? Hregs]" => /=.
+  iExists _. rewrite reg_col_cons. iFrame. iSplit; [done|]. iIntros "?".
+  iDestruct ("Hregs" with "[$]") as "$". iExists _. by iFrame.
+Qed.
+
 Fixpoint regcol_extract (r : reg_kind) (regs : list (reg_kind * valu_shape)) : option (valu_shape * list (reg_kind * valu_shape)) :=
   match regs with
   | (r', s)::regs' =>
@@ -1177,19 +1199,19 @@ Section instances.
     (find_in_context (FindRegMapsTo r) (λ rk,
       match rk with
       | RKMapsTo v' => (⌜v = v'⌝ -∗ r ↦ᵣ v' -∗ WPasm es)
-      | RKCol regs => tactic_hint (vm_compute_hint (list_find_idx (λ x, x.1 = KindReg r)) regs) (λ i,
-           (reg_col regs -∗ ⌜valu_has_shape v (regs !!! i).2⌝ -∗ WPasm es))
+      | RKCol regs =>
+          (tactic_hint (regcol_compute_hint (regcol_lookup (KindReg r)) regs) (λ s,
+             reg_col regs -∗ ⌜valu_has_shape v s⌝ -∗ WPasm es))
       end)) -∗
     WPasm (ReadReg r [] v ann :t: es).
   Proof.
-    unfold tactic_hint, vm_compute_hint.
+    unfold tactic_hint, regcol_compute_hint.
     iDestruct 1 as (rk) "[Hr Hwp]" => /=. case_match; simplify_eq.
     - by iApply (wp_read_reg with "Hr").
-    - iDestruct "Hwp" as (? [[??][?[??]]]%list_find_idx_Some) "Hwp"; simplify_eq/=.
-      erewrite list_lookup_total_correct; [|done].
-      iDestruct (big_sepL_lookup_acc with "Hr") as "[[%vact [% Hr]] Hregs]"; [done|] => /=.
-      iApply (wp_read_reg with "Hr"). iIntros "% Hr". subst. iApply ("Hwp" with "[-] [//]"). iApply "Hregs".
-      iExists _. by iFrame.
+    - iDestruct "Hwp" as (? ?) "Hwp"; simplify_eq/=.
+      iDestruct (regcol_lookup_Some with "Hr") as (??) "[Hr Hregs]"; [done|] => /=.
+      iApply (wp_read_reg with "Hr"). iIntros (?) "Hr". subst.
+      iApply ("Hwp" with "[-] [//]"). by iApply "Hregs".
   Qed.
 
   Lemma li_wp_read_reg_struct r f v ann es :
@@ -1244,20 +1266,19 @@ Section instances.
     (find_in_context (FindRegMapsTo r) (λ rk,
       match rk with
       | RKMapsTo v' => (⌜v = v'⌝ ∗ (r ↦ᵣ v' -∗ WPasm es))
-      | RKCol regs => tactic_hint (vm_compute_hint (list_find_idx (λ x, x.1 = KindReg r)) regs) (λ i,
-                      ⌜∀ v', valu_has_shape v' (regs !!! i).2 → v' = v⌝ ∗ (reg_col regs -∗ WPasm es))
+      | RKCol regs =>
+          (tactic_hint (regcol_compute_hint (regcol_lookup (KindReg r)) regs) (λ s,
+             ⌜∀ v', valu_has_shape v' s → v' = v⌝ ∗ (reg_col regs -∗ WPasm es)))
       end)) -∗
     WPasm (AssumeReg r [] v ann :t: es).
   Proof.
-    unfold tactic_hint, vm_compute_hint.
+    unfold tactic_hint, regcol_compute_hint.
     iDestruct 1 as (rk) "[Hr Hwp]" => /=. case_match; simplify_eq.
     - iDestruct "Hwp" as (->) "?". by iApply (wp_assume_reg with "Hr").
-    - iDestruct "Hwp" as (a [[??][?[??]]]%list_find_idx_Some Hr) "Hwp"; simplify_eq/=.
-      erewrite list_lookup_total_correct in Hr; [|done]; simplify_eq/=.
-      iDestruct (big_sepL_lookup_acc with "Hr") as "[[%vact [% Hr]] Hregs]"; [done|]; simplify_eq/=.
+    - iDestruct "Hwp" as (?? Hr) "Hwp"; simplify_eq/=.
+      iDestruct (regcol_lookup_Some with "Hr") as (vact ?) "[Hr Hregs]"; [done|] => /=.
       have ?: vact = v by naive_solver. subst.
-      iApply (wp_assume_reg with "Hr"). iIntros "Hr". iApply "Hwp". iApply "Hregs".
-      iExists _. by iFrame.
+      iApply (wp_assume_reg with "Hr"). iIntros "Hr". iApply "Hwp". by iApply "Hregs".
   Qed.
 
   Lemma li_wp_assume_reg_struct r f v ann es :
@@ -1465,22 +1486,22 @@ Section instances.
     (find_in_context (FindRegMapsTo r) (λ rk,
       match rk with
       | RKMapsTo v => (if v is RegVal_Base v' then r ↦ᵣ v -∗ Φ v' else False)
-      | RKCol regs => tactic_hint (vm_compute_hint (list_find_idx (λ x, x.1 = KindReg r)) regs) (λ i,
-        ∀ v, ⌜valu_has_shape v (regs !!! i).2⌝ -∗ ∃ v', ⌜v = RegVal_Base v'⌝ ∗ (reg_col regs -∗ Φ v')
+      | RKCol regs =>
+          tactic_hint (regcol_compute_hint (regcol_lookup (KindReg r)) regs) (λ s,
+           ∀ v, ⌜valu_has_shape v s⌝ -∗ ∃ v', ⌜v = RegVal_Base v'⌝ ∗ (reg_col regs -∗ Φ v')
              )
       end)) -∗
     WPaexp (AExp_Val (AVal_Var r []) ann) {{ Φ }}.
   Proof.
-    unfold tactic_hint, vm_compute_hint.
+    unfold tactic_hint, regcol_compute_hint.
     iDestruct 1 as (rk) "[Hr Hwp]" => /=. case_match; simplify_eq.
     - case_match => //; subst. by iApply (wpae_var_reg with "Hr").
-    - iDestruct "Hwp" as (i [[??][?[??]]]%list_find_idx_Some) "Hwp"; simplify_eq/=.
-      erewrite list_lookup_total_correct; [|done]; simplify_eq/=.
-      iDestruct (big_sepL_lookup_acc with "Hr") as "[[%vact [% Hr]] Hregs]"; [done|]; simplify_eq/=.
+    - iDestruct "Hwp" as (? ?) "Hwp"; simplify_eq/=.
+      iDestruct (regcol_lookup_Some with "Hr") as (??) "[Hr Hregs]"; [done|] => /=.
       iDestruct ("Hwp" with "[//]") as (? ->) "Hwp".
-      iApply (wpae_var_reg with "Hr"). iIntros "Hr". iApply "Hwp". iApply "Hregs".
-      iExists _. by iFrame.
+      iApply (wpae_var_reg with "Hr"). iIntros "Hr". iApply "Hwp". by iApply "Hregs".
   Qed.
+
   Lemma li_wpae_var_struct r f Φ ann :
     (find_in_context (FindStructRegMapsTo r f) (λ rk,
       match rk with
